Restore drfprops

src/prop/FutureCertify.v
@@ -23,11 +23,11 @@ Require Import Local.
 Require Import Thread.
 
 Require Import Cover.
-(* Require Import Mapping. *)
-(* Require Import Pred. *)
-(* Require Import Trace. *)
-(* Require Import MemoryProps. *)
-(* Require Import PFConsistent. *)
+Require Import Mapping.
+Require Import Pred.
+Require Import Trace.
+Require Import MemoryProps.
+Require Import PFConsistent.
 (* Require Import PFConsistentStrong. *)
 
 Set Implicit Arguments.
@@ -36,104 +36,105 @@ Module FutureCertify.
   Section FutureCertify.
     Variable (lang: language).
 
-    (* Lemma cap_steps_current_steps *)
-    (*       th0 th1 mem1 sc1 *)
-    (*       (LOCAL: Local.wf (Thread.local th0) (Thread.memory th0)) *)
-    (*       (MEMORY: Memory.closed (Thread.memory th0)) *)
-    (*       (SC: Memory.closed_timemap (Thread.sc th0) (Thread.memory th0)) *)
-    (*       (CAP: Memory.cap (Thread.memory th0) mem1) *)
-    (*       (SC_MAX: Memory.max_concrete_timemap mem1 sc1) *)
-    (*       (STEPS: rtc (@Thread.tau_step lang) *)
-    (*                   (Thread.mk lang (Thread.state th0) (Thread.local th0) sc1 mem1) *)
-    (*                   th1) *)
-    (*       (CONSISTENT: Local.promise_consistent (Thread.local th1)) *)
-    (*   : *)
-    (*     exists lc' sc' mem', *)
-    (*       (<<STEPS: rtc (@Thread.tau_step lang) *)
-    (*                     th0 *)
-    (*                     (Thread.mk lang (Thread.state th1) lc' sc' mem')>>) /\ *)
-    (*       (<<CONSISTENT: Local.promise_consistent lc'>>) *)
-    (* . *)
-    (* Proof. *)
-    (*   eapply pred_steps_thread_steps in STEPS. *)
-    (*   destruct th0, th1. ss. *)
-    (*   hexploit steps_map. *)
-    (*   { eapply ident_map_le. } *)
-    (*   { eapply ident_map_bot. } *)
-    (*   { eapply ident_map_eq. } *)
-    (*   { i. eapply ident_map_mappable_evt. } *)
-    (*   { eapply STEPS. } *)
-    (*   { ss. } *)
-    (*   { ss. } *)
-    (*   { ss. } *)
-    (*   { eapply Local.cap_wf; eauto. } *)
-    (*   { eapply LOCAL. } *)
-    (*   { eauto. } *)
-    (*   { eapply Memory.cap_closed; eauto. } *)
-    (*   { eauto. } *)
-    (*   { eapply Memory.max_concrete_timemap_closed; eauto. } *)
-    (*   { eapply map_ident_in_memory_local; eauto; ss. *)
-    (*     eapply ident_map_lt. *)
-    (*   } *)
-    (*   { econs. *)
-    (*     { i. destruct msg as [val released|]; auto. right. *)
-    (*       exists to, from, (Message.concrete val released), (Message.concrete val released). *)
-    (*       eapply Memory.cap_inv in GET; eauto. des; ss. esplits; eauto. *)
-    (*       { refl. } *)
-    (*       { eapply ident_map_message. } *)
-    (*       { refl. } *)
-    (*     } *)
-    (*     { i. eapply CAP in GET. left. exists fto, ffrom, fto, ffrom. splits; ss. *)
-    (*       { refl. } *)
-    (*       { refl. } *)
-    (*       { i. econs; eauto. } *)
-    (*     } *)
-    (*   } *)
-    (*   { eapply mapping_map_lt_collapsable_unwritable. eapply ident_map_lt. } *)
-    (*   { eapply ident_map_timemap. } *)
-    (*   { eapply Memory.max_concrete_timemap_spec; eauto. *)
-    (*     eapply Memory.cap_closed_timemap; eauto. } *)
-    (*   { instantiate (1:=fun _ => True). ss. } *)
-    (*   i. des. esplits. *)
-    (*   { eapply rtc_implies; try apply STEP. i. inv H. inv TSTEP. econs; eauto. } *)
-    (*   { inv LOCAL0. eapply promise_consistent_mon; cycle 1; eauto. *)
-    (*     { refl. } *)
-    (*     eapply promise_consistent_map; eauto. *)
-    (*     { eapply ident_map_le; eauto. } *)
-    (*     { eapply ident_map_eq; eauto. } *)
-    (*   } *)
-    (* Qed. *)
+    Lemma cap_steps_current_steps
+          th0 th1 mem1 sc1
+          (LOCAL: Local.wf (Thread.local th0) (Thread.memory th0))
+          (MEMORY: Memory.closed (Thread.memory th0))
+          (SC: Memory.closed_timemap (Thread.sc th0) (Thread.memory th0))
+          (CAP: Memory.cap (Thread.memory th0) mem1)
+          (SC_MAX: Memory.max_concrete_timemap mem1 sc1)
+          (STEPS: rtc (@Thread.tau_step lang)
+                      (Thread.mk lang (Thread.state th0) (Thread.local th0) sc1 mem1)
+                      th1)
+          (CONSISTENT: Local.promise_consistent (Thread.local th1))
+      :
+        exists lc' sc' mem',
+          (<<STEPS: rtc (@Thread.tau_step lang)
+                        th0
+                        (Thread.mk lang (Thread.state th1) lc' sc' mem')>>) /\
+          (<<CONSISTENT: Local.promise_consistent lc'>>)
+    .
+    Proof.
+      eapply pred_steps_thread_steps in STEPS.
+      destruct th0, th1. ss.
+      hexploit steps_map.
+      { eapply ident_map_le. }
+      { eapply ident_map_bot. }
+      { eapply ident_map_eq. }
+      { eapply ident_map_lt. }
+      { i. eapply ident_map_mappable_evt. }
+      { eapply STEPS. }
+      { ss. }
+      { ss. }
+      { ss. }
+      { eapply Local.cap_wf; eauto. }
+      { eapply LOCAL. }
+      { eauto. }
+      { eapply Memory.cap_closed; eauto. }
+      { eauto. }
+      { eapply Memory.max_concrete_timemap_closed; eauto. }
+      { eapply map_ident_in_memory_local; eauto; ss.
+        eapply ident_map_lt.
+      }
+      { econs.
+        { i. destruct msg as [val released|]; auto. right.
+          exists to, from, (Message.concrete val released), (Message.concrete val released).
+          eapply Memory.cap_inv in GET; eauto. des; ss. esplits; eauto.
+          { refl. }
+          { eapply ident_map_message. }
+          { refl. }
+        }
+        { i. eapply CAP in GET. left. exists fto, ffrom, fto, ffrom. splits; ss.
+          { refl. }
+          { refl. }
+          { i. econs; eauto. }
+        }
+      }
+      { eapply mapping_map_lt_collapsable_unwritable. eapply ident_map_lt. }
+      { eapply ident_map_timemap. }
+      { eapply Memory.max_concrete_timemap_spec; eauto.
+        eapply Memory.cap_closed_timemap; eauto. }
+      { instantiate (1:=fun _ => True). ss. }
+      i. des. esplits.
+      { eapply rtc_implies; try apply STEP. i. inv H. inv TSTEP. econs; eauto. }
+      { inv LOCAL0. eapply promise_consistent_mon; cycle 1; eauto.
+        { refl. }
+        eapply promise_consistent_map; eauto.
+        { eapply ident_map_le; eauto. }
+        { eapply ident_map_eq; eauto. }
+      }
+    Qed.
 
-    (* Definition future_certify lang (e:Thread.t lang): Prop := *)
-    (*   forall sc1 mem1 *)
-    (*     (FUTURE: Memory.future_weak (Thread.memory e) mem1) *)
-    (*     (FUTURE: TimeMap.le (Thread.sc e) sc1) *)
-    (*     (WF: Local.wf (Thread.local e) mem1) *)
-    (*     (SC: Memory.closed_timemap sc1 mem1) *)
-    (*     (MEM: Memory.closed mem1), *)
-    (*     (<<FAILURE: Thread.steps_failure (Thread.mk lang (Thread.state e) (Thread.local e) sc1 mem1)>>) \/ *)
-    (*     exists e2, *)
-    (*       (<<STEPS: rtc (@Thread.tau_step lang) (Thread.mk lang (Thread.state e) (Thread.local e) sc1 mem1) e2>>) /\ *)
-    (*       (<<PROMISES: (Local.promises (Thread.local e2)) = Memory.bot>>). *)
+    Definition future_certify lang (e:Thread.t lang): Prop :=
+      forall sc1 mem1
+        (FUTURE: Memory.future_weak (Thread.memory e) mem1)
+        (FUTURE: TimeMap.le (Thread.sc e) sc1)
+        (WF: Local.wf (Thread.local e) mem1)
+        (SC: Memory.closed_timemap sc1 mem1)
+        (MEM: Memory.closed mem1),
+        (<<FAILURE: Thread.steps_failure (Thread.mk lang (Thread.state e) (Thread.local e) sc1 mem1)>>) \/
+        exists e2,
+          (<<STEPS: rtc (@Thread.tau_step lang) (Thread.mk lang (Thread.state e) (Thread.local e) sc1 mem1) e2>>) /\
+          (<<PROMISES: (Local.promises (Thread.local e2)) = Memory.bot>>).
 
-    (* Lemma future_certify_exists *)
-    (*       e *)
-    (*       (LOCAL: Local.wf (Thread.local e) (Thread.memory e)) *)
-    (*       (MEMORY: Memory.closed (Thread.memory e)) *)
-    (*       (SC: Memory.closed_timemap (Thread.sc e) (Thread.memory e)) *)
-    (*       (CONSISTENT: @Thread.consistent lang e): *)
-    (*   future_certify e. *)
-    (* Proof. *)
-    (*   eapply consistent_pf_consistent_super_strong in CONSISTENT; eauto. des. *)
-    (*   exploit (@concrete_promise_max_timemap_exists (Thread.memory e) (Local.promises (Thread.local e))). *)
-    (*   { eapply MEMORY. } i. des. *)
-    (*   ii. exploit (CONSISTENT0 mem1 TimeMap.bot sc1); eauto. i. des. *)
-    (*   eapply Trace.silent_steps_tau_steps in STEPS; cycle 1. *)
-    (*   { eapply List.Forall_impl; eauto. i. ss. des. auto. } *)
-    (*   unguard. des. *)
-    (*   { left. unfold Thread.steps_failure. destruct e1. ss. esplits; eauto. } *)
-    (*   { right. esplits; eauto. } *)
-    (* Qed. *)
+    Lemma future_certify_exists
+          e
+          (LOCAL: Local.wf (Thread.local e) (Thread.memory e))
+          (MEMORY: Memory.closed (Thread.memory e))
+          (SC: Memory.closed_timemap (Thread.sc e) (Thread.memory e))
+          (CONSISTENT: @Thread.consistent lang e):
+      future_certify e.
+    Proof.
+      (* eapply consistent_pf_consistent_super_strong in CONSISTENT; eauto. des. *)
+      (* exploit (@concrete_promise_max_timemap_exists (Thread.memory e) (Local.promises (Thread.local e))). *)
+      (* { eapply MEMORY. } i. des. *)
+      (* ii. exploit (CONSISTENT0 mem1 TimeMap.bot sc1); eauto. i. des. *)
+      (* eapply Trace.silent_steps_tau_steps in STEPS; cycle 1. *)
+      (* { eapply List.Forall_impl; eauto. i. ss. des. auto. } *)
+      (* unguard. des. *)
+      (* { left. unfold Thread.steps_failure. destruct e1. ss. esplits; eauto. } *)
+      (* { right. esplits; eauto. } *)
+    Admitted
 
     Lemma future_consistent
           e sc' mem'
@@ -148,17 +149,13 @@ Module FutureCertify.
           (SC': Memory.closed_timemap sc' mem'):
       Thread.consistent (Thread.mk lang (Thread.state e) (Thread.local e) sc' mem').
     Proof.
-    (*   ii. ss. *)
-    (*   eapply future_certify_exists; try exact CONSISTENT; eauto. *)
-    (*   - etrans; eauto. eapply Memory.cap_future_weak; eauto. *)
-    (*   - etrans; eauto. *)
-    (*     hexploit Memory.cap_closed_timemap; try exact SC'; eauto. i. *)
-    (*     hexploit Memory.max_concrete_timemap_spec; eauto. *)
-    (*   - eapply Local.cap_wf; eauto. *)
-    (*   - eapply Memory.max_concrete_timemap_closed; eauto. *)
-    (*   - eapply Memory.cap_closed; eauto. *)
-    (* Qed. *)
-    Admitted.
+      ii. ss.
+      eapply future_certify_exists; try exact CONSISTENT; eauto.
+      - etrans; eauto. eapply Memory.cap_future_weak; eauto.
+      - eapply Local.cap_wf; eauto.
+      - eapply Memory.cap_closed_timemap; eauto.
+      - eapply Memory.cap_closed; eauto.
+    Qed.
   End FutureCertify.
 
   Lemma undef_added_failure lang st lc sc0 mem0 sc1 mem1
